src/Language/PlutusIR/Transform/SplitRec.v
@@ -3,8 +3,8 @@ From PlutusCert Require Import
   Analysis.FreeVars
   Analysis.Equality
   Analysis.UniqueBinders
+  Analysis.WellScoped
   Transform.Congruence
-  Static.Typing
   .
 Import NamedTerm.
 Import Term.
@@ -32,24 +32,32 @@ regrouping/reordering all bindings.
 Definition list_eq_elems {A} xs ys : Prop :=
   forall (x : A), In x xs <-> In x ys.
 
-(* Collect subsequent binding groups, together with the "inner" term *)
-Inductive collect_binding_groups : Term -> list Binding -> Term -> Prop :=
 
-  | cv_Let : forall t_body lets t_inner r bs,
-      collect_binding_groups t_body lets t_inner ->
-      collect_binding_groups (Let r bs t_body) (bs ++ lets) t_inner
+Definition min_Rec (r1 r2 : Recursivity) : Recursivity :=
+  match r1, r2 with
+    | NonRec, NonRec => NonRec
+    | _ , _ => Rec
+  end.
+
+(* Collect subsequent binding groups, together with the "inner" term and
+   minimum recursivity *)
+Inductive outer_binds : Term -> list Binding -> Term -> Recursivity -> Prop :=
+
+  | cv_Let : forall t_body lets t_inner r bs r_body,
+      outer_binds t_body lets t_inner r_body ->
+      outer_binds (Let r bs t_body) (bs ++ lets) t_inner (min_Rec r_body r)
 
   | cv_Other : forall t_inner,
-      collect_binding_groups t_inner [] t_inner
+      outer_binds t_inner [] t_inner NonRec
 
   .
 
 Inductive split_syn : Term -> Term -> Prop :=
-  | split_rec_let : forall bs t_body t bgs t_inner,
+  | split_rec_let : forall bs t_body t bgs t_inner min_rec,
 
       (* a decision-procedure would need to find the list bgs of binding groups that
          satisfies the second premise (needs to do backtracking) *)
-      collect_binding_groups t bgs t_inner ->
+      outer_binds t bgs t_inner min_rec ->
       list_eq_elems bs bgs ->
       split_syn t_body t_inner ->
       split_syn (Let Rec bs t_body) t
@@ -59,13 +67,13 @@ Inductive split_syn : Term -> Term -> Prop :=
       split_syn t t'
 .
 
-(* TODO: define and use well_scoped instead of well_typed *)
 Definition split_rec t t' :=
   split_syn t t' /\
-  well_typed t' /\
-  unique t.
+  unique t /\
+  closed t'
+.
 
 
-Definition collect_binding_groups_dec
+Definition outer_binds_dec
      : Term -> list binding_group * Term.
 Admitted.
